CpcMini/Lemmas.lean
@@ -18,7 +18,7 @@ set_option maxHeartbeats 10000000
    implication to be Boolean. -/
 theorem correct___eo_prog_scope (M : SmtModel) (x1 x2 : Term) :
   ((eo_interprets M x1 true) -> eo_interprets M x2 true) ->
-  (Not ((__eo_prog_scope x1 (Proof.pf x2)) = Term.Stuck)) ->
+  __eo_typeof (__eo_prog_scope x1 (Proof.pf x2)) = Term.Bool ->
   (eo_interprets M (__eo_prog_scope x1 (Proof.pf x2)) true) :=
 by
   sorry
@@ -27,7 +27,7 @@ by
 theorem correct___eo_prog_contra (M : SmtModel) (x1 x2 : Term) :
   (eo_interprets M x1 true) ->
   (eo_interprets M x2 true) ->
-  (Not ((__eo_prog_contra (Proof.pf x1) (Proof.pf x2)) = Term.Stuck)) ->
+  __eo_typeof (__eo_prog_contra (Proof.pf x1) (Proof.pf x2)) = Term.Bool ->
   (eo_interprets M (__eo_prog_contra (Proof.pf x1) (Proof.pf x2)) true) :=
 by
   sorry
@@ -37,7 +37,7 @@ by
    false as written: non-stuckness alone does not force the argument to have a
    semantic type on which equality is Boolean. -/
 theorem correct___eo_prog_refl (M : SmtModel) (x1 : Term) :
-  (Not ((__eo_prog_refl x1) = Term.Stuck)) ->
+  __eo_typeof (__eo_prog_refl x1) = Term.Bool ->
   (eo_interprets M (__eo_prog_refl x1) true) :=
 by
   sorry
@@ -55,7 +55,7 @@ by
 /- correctness theorem for __eo_prog_symm -/
 theorem correct___eo_prog_symm (M : SmtModel) (x1 : Term) :
   (eo_interprets M x1 true) ->
-  (Not ((__eo_prog_symm (Proof.pf x1)) = Term.Stuck)) ->
+  __eo_typeof (__eo_prog_symm (Proof.pf x1)) = Term.Bool ->
   (eo_interprets M (__eo_prog_symm (Proof.pf x1)) true) :=
 by
   sorry
@@ -63,7 +63,7 @@ by
 /- correctness theorem for __eo_prog_trans -/
 theorem correct___eo_prog_trans (M : SmtModel) (x1 : Term) :
   (eo_interprets M x1 true) ->
-  (Not ((__eo_prog_trans (Proof.pf x1)) = Term.Stuck)) ->
+  __eo_typeof (__eo_prog_trans (Proof.pf x1)) = Term.Bool ->
   (eo_interprets M (__eo_prog_trans (Proof.pf x1)) true) :=
 by
   sorry
